Addressed comments

src/Constants.ec
@@ -1,6 +1,7 @@
 pragma Goals:printall.
 
 require import AllCore.
+require import Field.
 require import Int.
 require import IntDiv.
 require import UInt256.
@@ -13,6 +14,11 @@ lemma Q_int: Q = W256.to_uint VerifierConsts.Q_MOD
     by rewrite /VerifierConsts.Q_MOD W256.of_uintK qE pmod_small; [trivial | reflexivity].
 lemma R_int: R = W256.to_uint VerifierConsts.R_MOD
     by rewrite /VerifierConsts.R_MOD W256.of_uintK rE pmod_small; [trivial | reflexivity].
+
+axiom q_eq_fieldq_p: Q = FieldQ.p.
+axiom r_eq_fieldr_p: R = FieldR.p.    
+lemma prime_q : prime Q by rewrite q_eq_fieldq_p; exact FieldQ.prime_p.
+lemma prime_r : prime R by rewrite r_eq_fieldr_p; exact FieldR.prime_p.
 
 (* 0x1dba8b5bdd64ef6ce29a9039aca3c0e524395c43b9227b96c75090cc6cc7ec97 *)
 op OMEGA : int = 13446667982376394161563610564587413125564757801019538732601045199901075958935 axiomatized by omegaE.
@@ -35,3 +41,16 @@ lemma non_residue_1_int: W256.to_uint VerifierConsts.NON_RESIDUES_1 = NON_RESIDU
   by rewrite /VerifierConsts.NON_RESIDUES_1 W256.of_uintK /NON_RESIDUE_1 pmod_small; [trivial | reflexivity].
 lemma non_residue_2_int: W256.to_uint VerifierConsts.NON_RESIDUES_2 = NON_RESIDUE_2
   by rewrite /VerifierConsts.NON_RESIDUES_2 W256.of_uintK /NON_RESIDUE_2 pmod_small; [trivial | reflexivity].
+
+op OMEGAFr = FieldR.inF OMEGA axiomatized by omegaFrE.
+op DOMAIN_SIZEFr = FieldR.inF DOMAIN_SIZE axiomatized by domain_sizeFrE.
+
+lemma omega_eq_omegaFr : FieldR.asint OMEGAFr = OMEGA. 
+proof.
+  rewrite omegaFrE FieldR.inFK /OMEGA -r_eq_fieldr_p /R. progress. 
+qed.
+
+lemma domain_eq_domainFr : FieldR.asint DOMAIN_SIZEFr = DOMAIN_SIZE.
+proof.
+  rewrite domain_sizeFrE FieldR.inFK /DOMAIN_SIZE -r_eq_fieldr_p /R. progress.
+qed.
