src/Field.ec
@@ -1,7 +1,6 @@
 pragma Goals:printall.
 
 require import AllCore.
-require import Constants.
 require import Int.
 require import IntDiv.
 require import StdOrder.
@@ -18,23 +17,5 @@ clone include ZModField
   rename "zmod" as "F"
   rename "ZModp" as "Zq".
 end FieldQ.
-
-axiom q_eq_fieldq_p: Q = FieldQ.p.
-axiom r_eq_fieldr_p: R = FieldR.p.    
-lemma prime_q : prime Q by rewrite q_eq_fieldq_p; exact FieldQ.prime_p.
-lemma prime_r : prime R by rewrite r_eq_fieldr_p; exact FieldR.prime_p.
   
 op (^) (x : FieldR.F) (k : int) = FieldR.exp x k axiomatized by RexpE.
-
-op OMEGAFr = FieldR.inF Constants.OMEGA axiomatized by omegaFrE.
-op DOMAIN_SIZEFr = FieldR.inF DOMAIN_SIZE axiomatized by domain_sizeFrE.
-
-lemma omega_eq_omegaFr : FieldR.asint OMEGAFr = OMEGA. 
-proof.
-  rewrite omegaFrE FieldR.inFK /OMEGA -r_eq_fieldr_p /Constants.R. progress. 
-qed.
-
-lemma domain_eq_domainFr : FieldR.asint DOMAIN_SIZEFr = DOMAIN_SIZE.
-proof.
-  rewrite domain_sizeFrE FieldR.inFK /DOMAIN_SIZE -r_eq_fieldr_p /Constants.R. progress.
-qed.
